src/cbor/pulse/raw/everparse/CBOR.Pulse.Raw.EverParse.SerializeCborEq.fst
@@ -10,6 +10,7 @@ friend CBOR.Spec.Raw.Format
 
 module F = CBOR.Spec.Raw.EverParse
 module LP = LowParse.Spec.Base
+module LPC = LowParse.Spec.Combinators
 
 open CBOR.Spec.Raw.Format
 open CBOR.Spec.Raw.EverParse
@@ -21,4 +22,24 @@ let serialize_cbor_eq_bare_serialize v =
      bare_serialize s v = s v
      So all four are definitionally equal. *)
   ()
+
+let pair_byte_compare_eq_cbor_compare_pair kv1 kv2 =
+  let s = serialize_raw_data_item in
+  let pair_ser = LPC.serialize_nondep_then s s in
+  (* Step 1: bare_serialize pair_ser kv == bare_serialize s (fst kv) ++ bare_serialize s (snd kv) *)
+  LPC.serialize_nondep_then_eq s s kv1;
+  LPC.serialize_nondep_then_eq s s kv2;
+  (* Step 2: bytes_lex_compare distributes over the concat (LowParse form;
+     SMTPat in CBOR.Spec.Raw.Format bridges to Format.bytes_lex_compare). *)
+  bytes_lex_compare_serialize_strong_prefix s
+    (fst kv1) (fst kv2)
+    (LP.bare_serialize s (snd kv1)) (LP.bare_serialize s (snd kv2));
+  (* Step 3: connect cbor_compare to Format.bytes_lex_compare on bare_serialize. *)
+  cbor_compare_correct (fst kv1) (fst kv2);
+  cbor_compare_correct (snd kv1) (snd kv2);
+  serialize_cbor_eq_bare_serialize (fst kv1);
+  serialize_cbor_eq_bare_serialize (fst kv2);
+  serialize_cbor_eq_bare_serialize (snd kv1);
+  serialize_cbor_eq_bare_serialize (snd kv2)
+
 
